snap

pulse/share/steel/examples/pulse/CustomSyntax.fst
@@ -12,171 +12,165 @@ open Pulse.Steel.Wrapper
 #push-options "--using_facts_from 'Prims FStar.Pervasives FStar.UInt FStar.UInt32 FStar.Ghost Pulse.Steel.Wrapper CustomSyntax'"
 #push-options "--ide_id_info_off"
 
-// ```pulse
-// fn test_write_10 (x:ref U32.t)
-//                  (#n:erased U32.t)
-//    requires pts_to x full_perm n
-//    ensures  pts_to x full_perm 0ul
-// {
-//     x := 1ul;
-//     x := 0ul;
-// }
-// ```
+```pulse
+fn test_write_10 (x:ref U32.t)
+                 (#n:erased U32.t)
+   requires pts_to x full_perm n
+   ensures  pts_to x full_perm 0ul
+{
+    x := 1ul;
+    x := 0ul;
+}
+```
+
+```pulse
+fn test_read (r:ref U32.t)
+             (#n:erased U32.t)
+             (#p:perm)
+   requires pts_to r p n
+   returns x : U32.t
+   ensures pts_to r p x
+{
+  let x = !r;
+  x
+}
+```
+
+```pulse
+fn swap (r1 r2:ref U32.t)
+        (#n1 #n2:erased U32.t)
+  requires 
+     (pts_to r1 full_perm n1 `star`
+      pts_to r2 full_perm n2)
+  ensures
+     (pts_to r1 full_perm n2 `star`
+      pts_to r2 full_perm n1)
+{
+  let x = !r1;
+  let y = !r2;
+  r1 := y;
+  r2 := x
+}
+```
+
+
+```pulse
+fn call_swap2 (r1 r2:ref U32.t)
+              (#n1 #n2:erased U32.t)
+   requires
+      (pts_to r1 full_perm n1 `star`
+       pts_to r2 full_perm n2)
+   ensures
+      (pts_to r1 full_perm n1 `star`
+       pts_to r2 full_perm n2)
+{
+   swap r1 r2;
+   swap r1 r2
+}
+```
+
+
+```pulse
+fn swap_with_elim_pure (r1 r2:ref U32.t) 
+                       (#n1 #n2:erased U32.t)
+   requires
+     (pts_to r1 full_perm n1 `star`
+      pts_to r2 full_perm n2)
+   ensures
+     (pts_to r1 full_perm n2 `star`
+      pts_to r2 full_perm n1)
+{
+   let x = !r1;
+   let y = !r2;
+   r1 := y;
+   r2 := x
+}
+```
+
+```pulse
+fn intro_pure_example (r:ref U32.t)
+                      (#n1 #n2:erased U32.t)
+   requires 
+     (pts_to r full_perm n1 `star`
+      pure (reveal n1 == reveal n2))
+   ensures 
+     (pts_to r full_perm n2 `star`
+      pure (reveal n2 == reveal n1))
+{
+  ()
+}
+```
+
+
+```pulse
+fn if_example (r:ref U32.t)
+              (n:(n:erased U32.t{U32.v (reveal n) == 1}))
+              (b:bool)
+   requires 
+     pts_to r full_perm n
+   ensures
+     pts_to r full_perm (U32.add (reveal n) 2ul)
+{
+   let x = read_atomic r;
+   if b
+   {
+     r := U32.add x 2ul
+   }
+   else
+   {
+     write_atomic r 3ul
+   }
+}
+```
+
 
 // ```pulse
-// fn test_read (r:ref U32.t)
-//              (#n:erased U32.t)
-//              (#p:perm)
-//    requires pts_to r p n
-//    returns x : U32.t
-//    ensures pts_to r p x
-// {
-//   !r
-// }
-// ```
-
-// ```pulse
-// fn swap (r1 r2:ref U32.t)
-//         (#n1 #n2:erased U32.t)
-//   requires 
-//      (pts_to r1 full_perm n1 `star`
-//       pts_to r2 full_perm n2)
-//   ensures
-//      (pts_to r1 full_perm n2 `star`
-//       pts_to r2 full_perm n1)
-// {
-//   let x = !r1;
-//   let y = !r2;
-//   r1 := y;
-//   r2 := x
-// }
-// ```
-
-// ```pulse
-// fn call_swap2 (r1 r2:ref U32.t)
-//               (#n1 #n2:erased U32.t)
-//    requires
-//       (pts_to r1 full_perm n1 `star`
-//        pts_to r2 full_perm n2)
-//    ensures
-//       (pts_to r1 full_perm n1 `star`
-//        pts_to r2 full_perm n2)
-// {
-//    swap r1 r2;
-//    swap r1 r2
-// }
-// ```
-
-// ```pulse
-// fn swap_with_elim_pure (r1 r2:ref U32.t) 
-//                        (#n1 #n2:erased U32.t)
-//    requires
-//      (pts_to r1 full_perm n1 `star`
-//       pts_to r2 full_perm n2)
-//    ensures
-//      (pts_to r1 full_perm n2 `star`
-//       pts_to r2 full_perm n1)
-// {
-//    let x = !r1;
-//    let y = !r2;
-//    r1 := y;
-//    r2 := x
-// }
-// ```
-
-// ```pulse
-// fn intro_pure_example (r:ref U32.t)
-//                       (#n1 #n2:erased U32.t)
+// ghost
+// fn elim_intro_exists2 (r:ref U32.t)
 //    requires 
-//      (pts_to r full_perm n1 `star`
-//       pure (reveal n1 == reveal n2))
+//      exists n. pts_to r full_perm n
 //    ensures 
-//      (pts_to r full_perm n2 `star`
-//       pure (reveal n2 == reveal n1))
+//      exists n. pts_to r full_perm n
 // {
-//   ()
-// }
-// ```
-
-// ```pulse
-// fn if_example (r:ref U32.t)
-//               (n:(n:erased U32.t{U32.v (reveal n) == 1}))
-//               (b:bool)
-//    requires 
-//      pts_to r full_perm n
-//    ensures
-//      pts_to r full_perm (U32.add (reveal n) 2ul)
-// {
-//    let x = read_atomic r;
-//    if b
-//    {
-//      r := U32.add x 2ul
-//    }
-//    else
-//    {
-//      write_atomic r 3ul
-//    }
-// }
-// ```
-
-// //
-// // THIS FAILS
-// //
-
-// // ```pulse
-// // ghost
-// // fn elim_intro_exists2 (r:ref U32.t)
-// //    requires 
-// //      exists n. pts_to r full_perm n
-// //    ensures 
-// //      exists n. pts_to r full_perm n
-// // {
-// //   introduce exists n. pts_to r full_perm n with _
-// // }
-// // ```
-
-
-// assume
-// val pred (b:bool) : vprop
-// assume
-// val read_pred (_:unit) (#b:erased bool)
-//     : stt bool (pred b) (fun r -> pred r)
-
-// ```pulse
-// fn while_test_alt (r:ref U32.t)
-//   requires 
-//     exists b n.
-//       (pts_to r full_perm n `star`
-//        pred b)
-//   ensures 
-//     exists n. (pts_to r full_perm n `star`
-//               pred false)
-// {
-//   while (read_pred())
-//   invariant b . exists n. (pts_to r full_perm n `star` pred b)
-//   {
-//     ()
-//   }
-// }
-// ```
-
-// ```pulse
-// fn infer_read_ex (r:ref U32.t)
-//   requires
-//     exists n. pts_to r full_perm n
-//   ensures exists n. pts_to r full_perm n
-// {
-//   let x = !r;
-//   ()
+//   introduce exists n. pts_to r full_perm n with _
 // }
 // ```
 
 
-// THIS FAILS
+assume
+val pred (b:bool) : vprop
+assume
+val read_pred (_:unit) (#b:erased bool)
+    : stt bool (pred b) (fun r -> pred r)
 
-// Probably, a pure vprop is left in the prover with
-//   a uvar
-// But the pure prop is of the form ?u == e
+```pulse
+fn while_test_alt (r:ref U32.t)
+  requires 
+    exists b n.
+      (pts_to r full_perm n `star`
+       pred b)
+  ensures 
+    exists n. (pts_to r full_perm n `star`
+              pred false)
+{
+  while (let x = read_pred(); x)
+  invariant b . exists n. (pts_to r full_perm n `star` pred b)
+  {
+    ()
+  }
+}
+```
+
+```pulse
+fn infer_read_ex (r:ref U32.t)
+  requires
+    exists n. pts_to r full_perm n
+  ensures exists n. pts_to r full_perm n
+{
+  let x = !r;
+  ()
+}
+```
 
 
 ```pulse
@@ -193,215 +187,231 @@ fn while_count2 (r:ref U32.t)
     let x = !r;
     if (x <^ 10ul)
     {
-      r := x +^ 1ul
+      r := x +^ 1ul; 
+      ()
     }
     else
     {
-      r := x -^ 1ul
+      r := x -^ 1ul;
+      ()
     }
-  }
+  };
+  ()
 }
 ```
 
 
-// // ```pulse
-// // fn test_par (r1 r2:ref U32.t)
-// //             (#n1 #n2:erased U32.t)
-// //   requires 
-// //     (pts_to r1 full_perm n1 `star`
-// //      pts_to r2 full_perm n2)
-// //   ensures
-// //     (pts_to r1 full_perm 1ul `star`
-// //      pts_to r2 full_perm 1ul)
-// // {
-// //   parallel
-// //   requires (pts_to r1 full_perm n1)
-// //        and (pts_to r2 full_perm n2)
-// //   ensures  (pts_to r1 full_perm 1ul)    
-// //        and (pts_to r2 full_perm 1ul)
-// //   {
-// //      r1 := 1ul
-// //   }
-// //   {
-// //      r2 := 1ul
-// //   };
-// //   ()
-// // }
-// // ```
+```pulse
+fn test_par (r1 r2:ref U32.t)
+            (#n1 #n2:erased U32.t)
+  requires 
+    (pts_to r1 full_perm n1 `star`
+     pts_to r2 full_perm n2)
+  ensures
+    (pts_to r1 full_perm 1ul `star`
+     pts_to r2 full_perm 1ul)
+{
+  parallel
+  requires (pts_to r1 full_perm n1)
+       and (pts_to r2 full_perm n2)
+  ensures  (pts_to r1 full_perm 1ul)    
+       and (pts_to r2 full_perm 1ul)
+  {
+     r1 := 1ul
+  }
+  {
+     r2 := 1ul
+  };
+  ()
+}
+```
 
-// // // A test for rewrite
-// // let mpts_to (r:ref U32.t) (n:erased U32.t) : vprop = pts_to r full_perm n
+// A test for rewrite
+let mpts_to (r:ref U32.t) (n:erased U32.t) : vprop = pts_to r full_perm n
 
-// // ```pulse
-// // fn rewrite_test (r:ref U32.t)
-// //                 (#n:erased U32.t)
-// //    requires (mpts_to r n)
-// //    ensures  (mpts_to r 1ul)
-// // {
-// //   rewrite (mpts_to r n) 
-// //        as (pts_to r full_perm n);
-// //   r := 1ul;
-// //   rewrite (pts_to r full_perm 1ul)
-// //        as (mpts_to r 1ul)
-// // }
-// // ```
+```pulse
+fn rewrite_test (r:ref U32.t)
+                (#n:erased U32.t)
+   requires (mpts_to r n)
+   ensures  (mpts_to r 1ul)
+{
+  rewrite (mpts_to r n) 
+       as (pts_to r full_perm n);
+  r := 1ul;
+  rewrite (pts_to r full_perm 1ul)
+       as (mpts_to r 1ul)
+}
+```
 
-// // ```pulse
-// // fn test_local (r:ref U32.t)
-// //               (#n:erased U32.t)
-// //    requires (pts_to r full_perm n)
-// //    ensures  (pts_to r full_perm 0ul)
-// // {
-// //   let mut x = 0ul;
-// //   let y = !x;
-// //   r := y;
-// //   introduce exists n. (pts_to x full_perm n) with _
-// // }
-// // ```
+```pulse
+fn test_local (r:ref U32.t)
+              (#n:erased U32.t)
+   requires (pts_to r full_perm n)
+   ensures  (pts_to r full_perm 0ul)
+{
+  let mut x = 0ul;
+  let y = !x;
+  r := y;
+  introduce exists n. (pts_to x full_perm n) with _
+}
+```
 
-// // ```pulse
-// // fn count_local (r:ref int) (n:int)
-// //    requires (pts_to r full_perm (hide 0))
-// //    ensures (pts_to r full_perm n)
-// // {
-// //   let mut i = 0;
-// //   while
-// //     (let m = !i; (m <> n))
-// //   invariant b. exists m. 
-// //     (pts_to i full_perm m `star`
-// //      pure (b == (m <> n)))
-// //   {
-// //     let m = !i;
-// //     i := m + 1;
-// //     ()
-// //   };
-// //   let x = !i;
-// //   r := x;
-// //   introduce exists m. (pts_to i full_perm m) with _
-// // }
-// // ```
+```pulse
+fn count_local (r:ref int) (n:int)
+   requires (pts_to r full_perm (hide 0))
+   ensures (pts_to r full_perm n)
+{
+  let mut i = 0;
+  while
+    (let m = !i; (m <> n))
+  invariant b. exists m. 
+    (pts_to i full_perm m `star`
+     pure (b == (m <> n)))
+  {
+    let m = !i;
+    i := m + 1;
+    ()
+  };
+  let x = !i;
+  r := x;
+  introduce exists m. (pts_to i full_perm m) with _
+}
+```
 
 
-// // let rec sum_spec (n:nat) : nat =
-// //   if n = 0 then 0 else n + sum_spec (n - 1)
+let rec sum_spec (n:nat) : nat =
+  if n = 0 then 0 else n + sum_spec (n - 1)
 
  
-// // let zero : nat = 0
+let zero : nat = 0
 
-// // ```pulse
-// // fn sum (r:ref nat) (n:nat)
-// //    requires exists i. (pts_to r full_perm i)
-// //    ensures (pts_to r full_perm (sum_spec n))
-// // {
-// //    let mut i = zero;
-// //    let mut sum = zero;
-// //    introduce exists b m s. (
-// //      pts_to i full_perm m `star`
-// //      pts_to sum full_perm s `star`
-// //      pure (s == sum_spec m /\
-// //            b == (m <> n)))
-// //    with (zero <> n);
+//
+// THIS FAILS
+//
+
+// ```pulse
+// fn sum (r:ref nat) (n:nat)
+//    requires exists i. (pts_to r full_perm i)
+//    ensures (pts_to r full_perm (sum_spec n))
+// {
+//    let mut i = zero;
+//    let mut sum = zero;
+//    introduce exists b m s. (
+//      pts_to i full_perm m `star`
+//      pts_to sum full_perm s `star`
+//      pure (s == sum_spec m /\
+//            b == (m <> n)))
+//    with (zero <> n);
         
-// //    while (let m = !i; (m <> n))
-// //    invariant b . exists m s. (
-// //      pts_to i full_perm m `star`
-// //      pts_to sum full_perm s `star`
-// //      pure (s == sum_spec m /\
-// //            b == (m <> n)))
-// //    {
-// //      let m = !i;
-// //      let s = !sum;
-// //      i := (m + 1);
-// //      sum := s + m + 1;
-// //      introduce exists b m s. (
-// //        pts_to i full_perm m `star`
-// //        pts_to sum full_perm s `star`
-// //        pure (s == sum_spec m /\
-// //              b == (m <> n)))
-// //      with (m + 1 <> n)
-// //    };
-// //    let s = !sum;
-// //    r := s;
-// //    introduce exists m. (pts_to i full_perm m) 
-// //    with _;
-// //    introduce exists s. (pts_to sum full_perm s)
-// //    with _
-// // }
-// // ```
+//    while (let m = !i; (m <> n))
+//    invariant b . exists m s. (
+//      pts_to i full_perm m `star`
+//      pts_to sum full_perm s `star`
+//      pure (s == sum_spec m /\
+//            b == (m <> n)))
+//    {
+//      let m = !i;
+//      let s = !sum;
+//      i := (m + 1);
+//      sum := s + m + 1;
+//      introduce exists b m s. (
+//        pts_to i full_perm m `star`
+//        pts_to sum full_perm s `star`
+//        pure (s == sum_spec m /\
+//              b == (m <> n)))
+//      with (m + 1 <> n)
+//    };
+//    let s = !sum;
+//    r := s;
+//    introduce exists m. (pts_to i full_perm m) 
+//    with _;
+//    introduce exists s. (pts_to sum full_perm s)
+//    with _
+// }
+// ```
 
-// // ```pulse
-// // fn sum2 (r:ref nat) (n:nat)
-// //    requires exists i. pts_to r full_perm i
-// //    ensures pts_to r full_perm (sum_spec n)
-// // {
-// //    let mut i = zero;
-// //    let mut sum = zero;
-// //    while (let m = !i; (m <> n))
-// //    invariant b . exists m s.
-// //      pts_to i full_perm m  **
-// //      pts_to sum full_perm s **
-// //      pure (s == sum_spec m /\ b == (m <> n))
-// //    {
-// //      let m = !i;
-// //      let s = !sum;
-// //      i := (m + 1);
-// //      sum := s + m + 1;
-// //      ()
-// //    };
-// //    let s = !sum;
-// //    r := s;
-// //    ()
-// // }
-// // ```
+//
+// ALSO FAILS
+// SAME REASON, uvars in eq2 props
+//
 
-// // ```pulse
-// // fn if_then_else_in_specs (r:ref U32.t)
-// //   requires `@(if true
-// //               then pts_to r full_perm 0ul
-// //               else pts_to r full_perm 1ul)
-// //   ensures  `@(if true
-// //               then pts_to r full_perm 1ul
-// //               else pts_to r full_perm 0ul)
-// // {
-// //   // need this for typechecking !r on the next line,
-// //   //   with inference of implicits
-// //   rewrite `@(if true then pts_to r full_perm 0ul else pts_to r full_perm 1ul)
-// //        as (pts_to r full_perm 0ul);
-// //   let x = !r;
-// //   r := U32.add x 1ul
-// // }
-// // ```
+// ```pulse
+// fn sum2 (r:ref nat) (n:nat)
+//    requires exists i. pts_to r full_perm i
+//    ensures pts_to r full_perm (sum_spec n)
+// {
+//    let mut i = zero;
+//    let mut sum = zero;
+//    while (let m = !i; (m <> n))
+//    invariant b . exists m s.
+//      pts_to i full_perm m  **
+//      pts_to sum full_perm s **
+//      pure (s == sum_spec m /\ b == (m <> n))
+//    {
+//      let m = !i;
+//      let s = !sum;
+//      i := (m + 1);
+//      sum := s + m + 1;
+//      ()
+//    };
+//    let s = !sum;
+//    r := s;
+//    ()
+// }
+// ```
 
-// // ```pulse
-// // fn test_tot_let (r:ref U32.t)
-// //   requires (pts_to r full_perm 0ul)
-// //   ensures  (pts_to r full_perm 2ul)
-// // {
-// //   let x = 1ul;
-// //   let y = 1ul;
-// //   r := U32.add x y
-// // }
-// // ```
+//
+// FAILS: refl_contains_uvar, unsupported reflection term
+//
 
-// // // Ascriptions coming in the way
-// // // ```pulse
-// // // fn if_then_else_in_specs2 (r:ref U32.t) (b:bool)
-// // //   requires (pts_to r full_perm (if b then 0ul else 1ul))
-// // //   ensures (pts_to r full_perm (if b then 1ul else 2ul))
-// // // {
-// // //   let x = !r;
-// // //   r := U32.add x 1ul
-// // // }
-// // // ```
+// ```pulse
+// fn if_then_else_in_specs (r:ref U32.t)
+//   requires `@(if true
+//               then pts_to r full_perm 0ul
+//               else pts_to r full_perm 1ul)
+//   ensures  `@(if true
+//               then pts_to r full_perm 1ul
+//               else pts_to r full_perm 0ul)
+// {
+//   // need this for typechecking !r on the next line,
+//   //   with inference of implicits
+//   rewrite `@(if true then pts_to r full_perm 0ul else pts_to r full_perm 1ul)
+//        as (pts_to r full_perm 0ul);
+//   let x = !r;
+//   r := U32.add x 1ul
+// }
+// ```
+
+```pulse
+fn test_tot_let (r:ref U32.t)
+  requires (pts_to r full_perm 0ul)
+  ensures  (pts_to r full_perm 2ul)
+{
+  let x = 1ul;
+  let y = 1ul;
+  r := U32.add x y
+}
+```
+
+// Ascriptions coming in the way
+// ```pulse
+// fn if_then_else_in_specs2 (r:ref U32.t) (b:bool)
+//   requires (pts_to r full_perm (if b then 0ul else 1ul))
+//   ensures (pts_to r full_perm (if b then 1ul else 2ul))
+// {
+//   let x = !r;
+//   r := U32.add x 1ul
+// }
+// ```
 
 
-// // ```pulse
-// // fn incr (x:nat)
-// //   requires emp
-// //   returns r : (r:nat { r > x })
-// //   ensures emp
-// // {
-// //   let y = x + 1;
-// //   ( y <: r:nat { r > x } )
-// // }
-// // ```
+```pulse
+fn incr (x:nat)
+  requires emp
+  returns r : (r:nat { r > x })
+  ensures emp
+{
+  let y = x + 1;
+  ( y <: r:nat { r > x } )
+}
+```
